Convert many proofs to llist2

src/llist.lean
@@ -10,35 +10,6 @@ namespace llist section
     def mem : V -> llist V -> Prop | x (P v) := x = v | x (L v l) := x = v ∨ mem x l
     instance has_mem_llist : has_mem V (llist V) := ⟨mem⟩
 
-    def mem2 (x : V) (l : llist2 V) : Prop := x = l.head ∨ x ∈ l.tail
-    instance has_mem_llist2 : has_mem V (llist2 V) := ⟨mem2⟩
-
-    def to_list2 (l : llist2 V) : list V := l.head :: l.tail
-    
-    def from_list2 : Π (l : list V), l ≠ [] -> llist2 V
-        | [] h := absurd rfl h
-        | (x::l) _ := ⟨x,l⟩
-
-    lemma ne_nil {l : llist2 V} : to_list2 l ≠ []
-        := by { trivial }
-
-    def size2             (l : llist2 V)                 : nat      := sizeof l.tail
-    def init2             (l : llist2 V)                 : list V   := list.init (to_list2 l)
-    def last2             (l : llist2 V)                 : V        := list.last (to_list2 l) ne_nil
-    def append2   (v : V) (l : llist2 V)                 : llist2 V := ⟨l.head, l.tail ++ [v]⟩
-    def nodup2            (l : llist2 V)                 : Prop     := list.nodup (to_list2 l)
-    def concat2           (l : llist2 V) (l' : llist2 V) : llist2 V := ⟨l.head, l.tail ++ l'.tail⟩
-    def map2 (f : V -> W) (l : llist2 V)                 : llist2 W := ⟨f l.head, list.map f l.tail⟩
-
-    def rev2 (l : llist2 V) : llist2 V := from_list2 (list.reverse (to_list2 l)) (ne_nil ∘ list.reverse_eq_nil.mp)
-
-    def inside2  : llist2 V -> list V | ⟨x,[]⟩ := []   | ⟨x,y::l⟩ := list.init (y::l)
-
-    inductive is_path2 : llist2 V -> Prop
-        | void {x}     : is_path2 ⟨x,[]⟩
-        | cons {x y l} : adj x y -> is_path2 ⟨y,l⟩ -> is_path2 ⟨x,y::l⟩
-
-
     def to_list :             llist V -> list V  |   (P v)    := [v]       |   (L v l)    := v :: to_list l
     def size    :             llist V -> nat     |   (P _)    := 0         |   (L v l)    := (size l) + 1
     def head    :             llist V -> V       |   (P v)    := v         |   (L v l)    := v
@@ -272,6 +243,298 @@ namespace llist section
     lemma last_map {f : V -> W} {l : llist V} : last (map f l) = f (last l)
         := by { induction l, refl, rwa [map,last,last] }
 end end llist
+
+namespace llist2 section
+    parameters {V W : Type} (adj : V -> V -> Prop)
+
+    lemma cases_on' {C : llist2 V -> Prop} (l : llist2 V)
+                (h0 : ∀ {x}, C ⟨x,[]⟩) (h1 : ∀ {x y ys}, C ⟨x,y::ys⟩) : C l 
+        := by { cases l with x l, cases l, exact h0, exact h1 }
+
+    lemma induction_on {C : llist2 V → Prop} (l : llist2 V)
+                (H0 : ∀ {x}, C ⟨x,[]⟩) (H1 : ∀ {x y ys} (hr : C ⟨y,ys⟩), C ⟨x,y::ys⟩) : C l 
+        := by { cases l with x l, induction l with y l hr generalizing x,
+            { exact H0 },
+            { exact H1 (hr y) } }
+
+    def mem (x : V) (l : llist2 V) : Prop := x = l.head ∨ x ∈ l.tail
+    instance : has_mem V (llist2 V) := ⟨mem⟩
+
+    instance : has_well_founded (llist2 V) := ⟨_, measure_wf ((λ n, n+n) ∘ list.length ∘ llist2.tail)⟩
+
+    def to_list (l : llist2 V) : list V := l.head :: l.tail
+    
+    def from_list : Π (l : list V), l ≠ [] -> llist2 V
+        | [] h := absurd rfl h
+        | (x::l) _ := ⟨x,l⟩
+
+    lemma ne_nil {l : llist2 V} : to_list l ≠ []
+        := by { trivial }
+
+    def size2             (l : llist2 V)                 : nat      := sizeof l.tail
+    def cons      (v : V) (l : llist2 V)                 : llist2 V := ⟨v,l.head::l.tail⟩
+    def append    (v : V) (l : llist2 V)                 : llist2 V := ⟨l.head, l.tail ++ [v]⟩
+    def concat            (l : llist2 V) (l' : llist2 V) : llist2 V := ⟨l.head, l.tail ++ l'.tail⟩
+    def map2 (f : V -> W) (l : llist2 V)                 : llist2 W := ⟨f l.head, list.map f l.tail⟩
+
+    def reverse : llist2 V -> llist2 V | ⟨x,[]⟩ := ⟨x,[]⟩ | ⟨x,y::l⟩ := append x (reverse ⟨y,l⟩)
+    def last    : llist2 V -> V        | ⟨x,[]⟩ := x      | ⟨x,y::l⟩ := last ⟨y,l⟩
+    def is_path : llist2 V -> Prop     | ⟨x,[]⟩ := true   | ⟨x,y::l⟩ := adj x y ∧ is_path ⟨y,l⟩
+    def nodup   : llist2 V -> Prop     | ⟨x,[]⟩ := true   | ⟨x,y::l⟩ := x ∉ llist2.mk y l ∧ nodup ⟨y,l⟩
+    def init    : llist2 V -> list V   | ⟨x,[]⟩ := []     | ⟨x,y::l⟩ := x :: init ⟨y,l⟩
+    def inside  : llist2 V -> list V   | ⟨x,[]⟩ := []     | ⟨x,y::l⟩ := init ⟨y,l⟩
+
+    @[simp] def compat (l₁ l₂ : llist2 V) := last l₁ = head l₂
+
+    variables {x y v w : V} {l l' l'' : llist2 V} {xs ys zs : list V}
+
+    @[simp] lemma head_concat : head (concat l l') = head l
+        := rfl
+
+    lemma last_is_last : last ⟨x,xs⟩ = list.last (to_list ⟨x,xs⟩) ne_nil
+        := by { induction xs with y ys hr generalizing x,
+            { simp [last,to_list] },
+            { simp [last,to_list], exact hr } }
+
+    lemma last_of_ne_nil {h : ys ≠ []} : last ⟨x,ys⟩ = list.last ys h
+        := by { cases ys with y ys, contradiction, simp [last], exact last_is_last }
+
+    lemma last_of_ne_nil' {h : ys ≠ []} : last ⟨x,xs++ys⟩ = list.last ys h
+        := by { induction xs generalizing x,
+            { cases ys, contradiction, simp [last], exact last_is_last },
+            { simp [last], exact xs_ih } }
+
+    @[simp] lemma last_concat (h : compat l l') : last (concat l l') = last  l'
+        := by { cases l' with x' l', cases l' with y' l',
+            { simp [concat,last] at h ⊢, convert h, cases l, refl },
+            { simp [concat,last_of_ne_nil,last_of_ne_nil'] } }
+
+    @[simp] lemma head_append : head (append v l) = head l
+        := rfl
+
+    @[simp] lemma last_append : last (append v l) = v
+        := by { cases l with x l, simp [append,last,last_of_ne_nil'] }
+
+    @[simp] lemma rev_append : reverse (append v l) = cons v (reverse l)
+        := by { apply induction_on l; intros, refl, 
+            simp [append,reverse] at hr ⊢, rw hr, finish }
+
+    @[simp] lemma rev_head : head (reverse l) = last l
+        := by { apply induction_on l; intros, refl, simp [reverse,append,hr,last] }
+
+    @[simp] lemma rev_last : last (reverse l) = head l
+        := by { apply cases_on' l; intros, refl, rw [reverse,last_append] }
+
+    @[simp] lemma rev_rev : reverse (reverse l) = l
+        := by { apply induction_on l; intros, refl, rw [reverse,rev_append,hr], refl }
+
+    lemma mem_iff : x ∈ l <-> x = head l ∨ x ∈ tail l
+        := by { trivial }
+
+    @[simp] lemma mem_singleton : x ∈ (⟨y,[]⟩ : llist2 V) <-> x = y
+        := by { simp [mem_iff] }
+
+    @[simp] lemma mem_cons : x ∈ (⟨v,xs⟩ : llist2 V) <-> x = v ∨ x ∈ xs
+        := mem_iff
+
+    @[simp] lemma concat_path (h : compat l l') : is_path (concat l l') <-> is_path l ∧ is_path l'
+        := by { revert h, apply induction_on l; intros, 
+            { simp [is_path,concat,last] at h ⊢, subst h, cases l', trivial }, 
+            { simp [concat,is_path] at hr h ⊢, rw [hr h,and.assoc] } }
+
+    @[simp] lemma mem_append : w ∈ append v l <-> w = v ∨ w ∈ l
+        := by { apply induction_on l; { intros, rw append, finish } }
+
+    @[simp] lemma mem_rev : v ∈ reverse l <-> v ∈ l
+        := by { apply induction_on l; intros, simp [reverse], simp [reverse,mem_append,hr] }
+
+    @[simp] lemma mem_head : head l ∈ l
+        := by { left, refl }
+
+    @[simp] lemma mem_last : last l ∈ l
+        := by { apply induction_on l; intros, { left, refl }, { right, assumption } }
+
+    @[simp] lemma mem_list : x ∈ to_list l <-> x ∈ l
+        := by { apply induction_on l; intros; simp [to_list] }
+
+    @[simp] lemma append_nodup : nodup (append x l) <-> x ∉ l ∧ nodup l
+        := by { apply induction_on l; intros, { simp [append,nodup], finish },
+            { simp [nodup,append] at hr ⊢, rw hr, finish } }
+
+    @[simp] lemma rev_nodup : nodup (reverse l) <-> nodup l
+        := by { apply induction_on l; intros, { finish }, { simp [reverse,hr,nodup] } }
+
+    @[simp] lemma append_is_path : is_path (append v l) <-> adj (last l) v ∧ is_path l
+        := by { apply induction_on l; intros, { simp [append,is_path,last] }, 
+            { simp [append,is_path,last] at hr ⊢, rw hr, finish } }
+
+    @[simp] lemma init_append : init (append x l) = to_list l
+        := by { apply induction_on l; intros, refl, { simp [append,init,to_list] at hr ⊢, exact hr } }
+
+    @[simp] lemma list_head_tail : head l :: tail l = to_list l
+        := rfl
+
+    @[simp] lemma list_init_last : init l ++ [last l] = to_list l
+        := by { apply induction_on l; intros, refl, rw [init,last,to_list], finish }
+
+    @[simp] lemma list_head_init' : v :: inside (cons v l) = init (cons v l)
+        := by { apply induction_on l; intros, refl, simp [cons,inside,init] }
+
+    @[simp] lemma list_head_init (h : l.tail ≠ []) : head l :: inside l = init l
+        := by { revert h, apply cases_on' l; intros, contradiction, refl }
+
+    @[simp] lemma list_tail_last' : inside (cons v l) ++ [last (cons v l)] = tail (cons v l)
+        := by { rw [cons,inside,last,list_init_last], refl }
+
+    @[simp] lemma list_tail_last (h : l.tail ≠ []) : inside l ++ [last l] = tail l
+        := by { cases l with x l, cases l, contradiction, simp [inside,last,to_list] }
+
+    @[simp] lemma init_inside (h : l.tail ≠ []) : init l = (head l) :: inside l
+        := by { revert h, apply induction_on l; intros, contradiction, simp [init,inside] }
+
+    @[simp] lemma inside_append : inside (append x l) = tail l
+        := by { apply induction_on l; intros, refl, simp [append,inside] at hr ⊢, assumption }
+
+    @[simp] lemma tail_append : (append x l).tail = tail l ++ [x]
+        := by { apply induction_on l; intros, refl, simp [append] }
+
+    @[simp] lemma tail_rev : tail (reverse l) = list.reverse (init l)
+        := by { apply induction_on l; intros, refl, simp [reverse], rw hr, simp [inside] }
+
+    @[simp] lemma rev_inside : inside (reverse l) = list.reverse (inside l)
+        := by { apply cases_on' l; intros, refl, simp [reverse,inside] } 
+
+    @[simp] lemma rev_is_path (h : symmetric adj) : is_path (reverse l) <-> is_path l
+        := by { apply induction_on l; intros, trivial, rw [reverse,append_is_path,hr], simp [is_path],
+            exact and_congr ⟨@h _ _, @h _ _⟩ iff.rfl }
+
+    @[simp] lemma mem_concat (h : compat l l') : x ∈ concat l l' <-> x ∈ l ∨ x ∈ l'
+        := by { split,
+            { intro h, cases h, 
+                { left, left, assumption },
+                { rw [concat,list.mem_append] at h_1, cases h_1, 
+                    { left, right, assumption },
+                    { right, right, assumption } } },
+            { intro h, cases h,
+                { cases h_1,
+                    { left, assumption },
+                    { right, rw [concat,list.mem_append], left, assumption } },
+                { cases h_1,
+                    { rw [compat] at h, rw [h_1,<-h], apply cases_on' l; intros,
+                        { left, refl }, 
+                        { right, simp [last], set z := last (⟨y,ys⟩ : llist2 V),
+                            have h0 : z ∈ (⟨y,ys⟩ : llist2 V) := mem_last, cases h0,
+                                { left, exact h0 },
+                                { simp [concat], right, left, exact h0 } } },
+                    { right, simp [concat], right, assumption } } } }
+
+    @[simp] lemma concat_nil (h : last l = w) : concat l ⟨w,[]⟩ = l
+        := by { revert h, apply cases_on' l; intros, refl, simp [concat] }
+
+    @[simp] lemma concat_nil2                      : concat (P w) l           = l
+        := rfl
+
+    @[simp] lemma concat_size                      : size (concat l l')       = size l + size l'
+        := by { induction l; rw [concat,size], { norm_num }, { rw [l_ih,size], norm_num } }
+
+    lemma         concat_assoc                     : concat (concat l l') l'' = concat l (concat l' l'')
+        := by { induction l; rw [concat,concat], rw [l_ih,concat] }
+
+    lemma         concat_nodup   (h : compat l l') : nodup (concat l l')    <-> nodup l ∧ nodup l' ∧ (∀ x, x ∈ l ∧ x ∈ l' -> x = head l')
+        := by { induction l with v v l hr; rw [concat,nodup],
+            { split, { intro, refine ⟨trivial,a,_⟩, intros x h1, rw mem_singleton at h1, rwa h1.1 }, tauto },
+            { rw [nodup,hr h], rw [compat,last] at h, split,
+                { rintros ⟨h1,h2,h3,h4⟩, rw mem_concat h at h1, push_neg at h1, refine ⟨⟨h1.1,h2⟩,h3,_⟩,
+                    rintros x ⟨h6,h7⟩, cases h6,
+                    { subst h6, cases h1.2 h7 },
+                    { exact h4 x ⟨h6,h7⟩ } },
+                { rintros ⟨⟨h1,h2⟩,h3,h4⟩, rw mem_concat h, push_neg, refine ⟨⟨h1,_⟩,h2,h3,_⟩,
+                    { intro h5, have h6 := h4 v ⟨(or.inl rfl),h5⟩, subst h6, rw <-h at h1, exact (h1 mem_last) },
+                    { rintros x ⟨h5,h6⟩, exact h4 x ⟨(or.inr h5),h6⟩ } } } }
+
+    lemma         mem_iff             (h : l = l') : x ∈ l                  <-> x ∈ l'
+        := by { rw h }
+
+    lemma         mem_init        (h : x ∈ init l) : x ∈ l
+        := by { induction l, cases h, cases h, exact or.inl h, exact or.inr (l_ih h) }
+
+    lemma         mem_head_init'                   : v ∈ init (L v l)
+        := by { rw [init], left, refl }
+
+    lemma         mem_head_init   (h : 0 < size l) : head l ∈ init l
+        := by { cases l, cases h, exact mem_head_init' }
+
+    lemma         mem_last_tail   (h : 0 < size l) : last l ∈ tail l
+        := by { cases l, cases h, clear h, rw [last,tail], induction l_a_1,
+            { left, refl }, { rw [last,head,tail], right, assumption } }
+
+    lemma         mem_tail        (h : x ∈ tail l) : x ∈ l
+        := by { cases l, cases h, rw [tail,list_head_tail,mem_list] at h, right, assumption }
+
+    lemma         mem_init_last                    : x ∈ l                  <-> x ∈ init l ∨ x = last l
+        := by { split,
+            { intro, induction l, { right, assumption }, { cases a, { left, left, exact a },
+                cases l_ih a, { left, right, assumption }, { right, rwa last } } },
+            { intro, cases a, exact mem_init a, convert mem_last } }
+
+    lemma         mem_head_tail                    : x ∈ l                  <-> x = head l ∨ x ∈ tail l
+        := by { cases l, { rw [mem_singleton,head,tail], convert (or_false _).symm },
+            { rw [head,tail,list_head_tail,mem_list,mem_cons] } }
+
+    lemma         mem_init_inside'                 : x ∈ init (L v l)       <-> x = v ∨ x ∈ inside (L v l)
+        := by { rw [init,inside,list.mem_cons_iff] }
+
+    lemma         mem_init_inside (h : 0 < size l) : x ∈ init l             <-> x = head l ∨ x ∈ inside l
+        := by { rw [<-(list_head_init h),list.mem_cons_iff] }
+
+    lemma         mem_tail_inside'                 : x ∈ tail (L v l)       <-> x ∈ inside (L v l) ∨ x = last l
+        := by { rw [inside,<-mem_init_last,tail,mem_head_tail], trivial }
+
+    lemma         mem_tail_inside (h : 0 < size l) : x ∈ tail l             <-> x ∈ inside l ∨ x = last l
+        := by { rw [<-(list_tail_last h),list.mem_append_eq,list.mem_singleton] }
+
+    lemma         nodup_mem_head     (h : nodup l) : head l ∉ tail l
+        := by { cases l, { rw [tail,list.mem_nil_iff], trivial }, 
+            { rw [head,tail,list_head_tail,mem_list], exact h.1 } }
+
+    lemma         nodup_mem_last     (h : nodup l) : last l ∉ init l
+        := by { induction l, { rw [init,list.mem_nil_iff], trivial }, 
+            { rw [last,init,list.mem_cons_iff], push_neg, split,
+                { intro, apply h.1, convert mem_last, exact a.symm },
+                { exact l_ih h.2 } } }
+
+    lemma         rev_compat                       : compat l l' <-> compat l'.rev l.rev
+        := by { rw [compat,compat,rev_last,rev_head,eq_comm] }
+
+    lemma         concat_append                    : append v (concat l l')  = concat l (append v l')
+        := by { induction l; rw [concat,concat], rw [append,l_ih] }
+
+    lemma         rev_concat     (h : compat l l') : rev (concat l l')       = concat (rev l') (rev l)
+        := by { induction l,
+            { rw [concat,rev,concat_nil], rw [rev_last], exact h.symm },
+            { rw [concat,rev,l_ih h,concat_append,rev] } }
+
+    lemma         nodup_init         (h : nodup l) : list.nodup (init l)
+        := by { induction l, { exact list.pairwise.nil }, 
+            { rw [init,list.nodup,list.pairwise_cons], refine ⟨_,l_ih h.2⟩, 
+                intros a h1 h2, replace h := h.1, rw h2 at h, exact h (mem_init h1) } }
+
+    lemma         nodup_of_init : list.nodup (init l) -> last l ∉ init l -> nodup l
+        := by { induction l, { intros, trivial },
+            { rw [init,last,nodup,list.nodup_cons,list.mem_cons_iff], push_neg, 
+                rintros ⟨h1,h2⟩ ⟨h3,h4⟩, refine ⟨_,l_ih h2 h4⟩,
+                rw mem_init_last, push_neg, exact ⟨h1,h3.symm⟩ } }
+end end llist2
+
+namespace llist2 section
+    parameters {V W : Type}
+
+    lemma head_map {f : V -> W} {l : llist V} : head (map f l) = f (head l)
+        := by { cases l; refl }
+
+    lemma last_map {f : V -> W} {l : llist V} : last (map f l) = f (last l)
+        := by { induction l, refl, rwa [map,last,last] }
+end end llist2
 
 @[ext] structure llist' (V : Type) (x y : V) := (l : llist V) (hx : l.head = x) (hy : l.last = y)
 instance {V : Type} {x y : V} : has_coe (llist' V x y) (llist V) := ⟨llist'.l⟩
